put assume in ge_mod and sub_mod

lib/bv32_mm_lemmas.i.dfy
@@ -138,4 +138,80 @@ module bv32_mm_lemmas refines generic_mm_lemmas {
         GBV.BVSEQ.SeqZero(NUM_WORDS)
     }
 
+    datatype mp_vars = mp_vars(
+        mp_frame_ptr: uint32, // writable
+        mm_frame_ptr: uint32, // writable
+        mma_frame_ptr: uint32, // writable
+        iter_rr: iter_t, 
+        iter_n: iter_t,
+        iter_in: iter_t,
+        iter_ar: iter_t, // writable
+        iter_aar: iter_t, // writable
+        iter_out: iter_t // writable
+    )
+
+    predicate mp_vars_inv(
+        vars: mp_vars,
+        mem: mem_t,
+        rr_ptr: nat,
+        n_ptr: nat,
+        in_ptr: nat,
+        ar_ptr: nat,
+        aar_ptr: nat,
+        out_ptr: nat,
+        rsa: rsa_params)
+    {
+        && valid_frame_ptr(mem, vars.mp_frame_ptr, 8)
+        && valid_frame_ptr(mem, vars.mm_frame_ptr, 8)
+        && valid_frame_ptr(mem, vars.mma_frame_ptr, 12)
+
+        && mvar_iter_inv(mem, vars.iter_rr, rr_ptr, 0, rsa.RR)
+        && mvar_iter_inv(mem, vars.iter_n, n_ptr, 0, rsa.M)
+        && mvar_iter_inv(mem, vars.iter_in, in_ptr, 0, rsa.SIG)
+        && mvar_iter_inv(mem, vars.iter_ar, ar_ptr, 0, NA)
+        && mvar_iter_inv(mem, vars.iter_aar, aar_ptr, 0, NA)
+        && mvar_iter_inv(mem, vars.iter_out, out_ptr, 0, NA)
+
+        && vars.iter_ar.base_addr != vars.iter_rr.base_addr
+        && vars.iter_ar.base_addr != vars.iter_n.base_addr
+        && vars.iter_ar.base_addr != vars.iter_in.base_addr
+        && vars.iter_ar.base_addr != vars.iter_aar.base_addr
+        && vars.iter_ar.base_addr != vars.iter_out.base_addr
+        && vars.iter_ar.base_addr != vars.mp_frame_ptr
+        && vars.iter_ar.base_addr != vars.mm_frame_ptr
+        && vars.iter_ar.base_addr != vars.mma_frame_ptr
+
+        && vars.iter_aar.base_addr != vars.iter_rr.base_addr
+        && vars.iter_aar.base_addr != vars.iter_n.base_addr
+        && vars.iter_aar.base_addr != vars.iter_in.base_addr
+        && vars.iter_aar.base_addr != vars.iter_out.base_addr
+        && vars.iter_aar.base_addr != vars.mp_frame_ptr
+        && vars.iter_aar.base_addr != vars.mm_frame_ptr
+        && vars.iter_aar.base_addr != vars.mma_frame_ptr
+
+        && vars.iter_out.base_addr != vars.iter_rr.base_addr
+        && vars.iter_out.base_addr != vars.iter_n.base_addr
+        && vars.iter_out.base_addr != vars.iter_in.base_addr
+        && vars.iter_out.base_addr != vars.mp_frame_ptr
+        && vars.iter_out.base_addr != vars.mm_frame_ptr
+        && vars.iter_out.base_addr != vars.mma_frame_ptr
+
+        && vars.mp_frame_ptr != vars.iter_rr.base_addr
+        && vars.mp_frame_ptr != vars.iter_n.base_addr
+        && vars.mp_frame_ptr != vars.iter_in.base_addr
+        && vars.mp_frame_ptr != vars.mm_frame_ptr
+        && vars.mp_frame_ptr != vars.mma_frame_ptr
+
+        && vars.mm_frame_ptr != vars.iter_rr.base_addr
+        && vars.mm_frame_ptr != vars.iter_n.base_addr
+        && vars.mm_frame_ptr != vars.iter_in.base_addr
+        && vars.mm_frame_ptr != vars.mma_frame_ptr
+
+        && vars.mma_frame_ptr != vars.iter_rr.base_addr
+        && vars.mma_frame_ptr != vars.iter_n.base_addr
+        && vars.mma_frame_ptr != vars.iter_in.base_addr
+
+        && rsa_params_inv(rsa)
+    }
+
 }
